Test/inst/inst1.bpl
@@ -11,9 +11,9 @@ procedure INV0(n: int)
 
   assume 0 <= i;
   assume i <= n;
-  assume (forall {:inst_at "A"} pa: PA :: PAs[pa] == if is#ADD(pa) && i < i#ADD(pa) && i#ADD(pa) <= n then 1 else 0);
-  assume (forall {:inst_at "A"} pa: PA :: PAs[pa] == 0);
-  assert {:inst_add "A", ADD(n)} i == n;
+  assume (forall {:inst_at "A0"} pa: PA :: PAs[pa] == if is#ADD(pa) && i < i#ADD(pa) && i#ADD(pa) <= n then 1 else 0);
+  assume (forall {:inst_at "A0"} pa: PA :: PAs[pa] == 0);
+  assert {:inst_add "A0", ADD(n)} i == n;
 }
 
 procedure INV1(n: int)
@@ -24,11 +24,11 @@ procedure INV1(n: int)
 
   assume 0 <= i;
   assume i <= n;
-  assume (forall {:inst_at "A"} pa: PA :: PAs[pa] == if is#ADD(pa) && i < i#ADD(pa) && i#ADD(pa) <= n then 1 else 0);
-  assume (forall {:inst_at "A"} pa: PA :: PAs[pa] == 0);
+  assume (forall {:inst_at "A1"} pa: PA :: PAs[pa] == if is#ADD(pa) && i < i#ADD(pa) && i#ADD(pa) <= n then 1 else 0);
+  assume (forall {:inst_at "A1"} pa: PA :: PAs[pa] == 0);
   m := n + 1;
   m := m + 1;
-  assert {:inst_add "A", ADD(m-2)} i == n;
+  assert {:inst_add "A1", ADD(m-2)} i == n;
 }
 
 procedure INV2(n: int)
@@ -38,7 +38,30 @@ procedure INV2(n: int)
 
   assume 0 <= i;
   assume i <= n;
-  PAs := (lambda {:inst_at "A"} pa: PA :: if is#ADD(pa) && i < i#ADD(pa) && i#ADD(pa) <= n then 1 else 0);
-  assume (forall {:inst_at "A"} pa: PA :: PAs[pa] == 0);
-  assert {:inst_add "A", ADD(n)} i == n;
+  PAs := (lambda {:inst_at "A2"} pa: PA :: {:labels "A2"} if is#ADD(pa) && i < i#ADD(pa) && i#ADD(pa) <= n then 1 else 0);
+  assume (forall pa: PA :: PAs[pa] == 0);
+  assert {:inst_add "A2", ADD(n)} i == n;
+}
+
+procedure INV3(n: int)
+{
+  var i: int;
+  var PAs: [PA]int;
+
+  assume 0 <= i;
+  assume i <= n;
+
+  call PAs := CreateLambda(i, n);
+  call LookupLambda(i, n, PAs);
+}
+
+procedure {:inline 1} CreateLambda(i: int, n: int) returns (PAs: [PA]int)
+{
+  PAs := (lambda {:inst_at "A3"} pa: PA :: {:labels "A3"} if is#ADD(pa) && i < i#ADD(pa) && i#ADD(pa) <= n then 1 else 0);
+}
+
+procedure {:inline 1} LookupLambda(i: int, n: int, PAs: [PA]int)
+{
+  assume (forall pa: PA :: PAs[pa] == 0);
+  assert {:inst_add "A3", ADD(n)} i == n;
 }
